src/program_proof/pav/test.v
@@ -1,8 +1,7 @@
 From Perennial.program_proof Require Import grove_prelude.
 From Goose.github_com.mit_pdos.pav Require Import kt.
 
-From iris.base_logic Require Import mono_nat.
-From Perennial.program_proof.pav Require Import advrpc auditor basictest core client cryptoffi history rpc serde server.
+From Perennial.program_proof.pav Require Import advrpc auditor core client cryptoffi history rpc serde server test_helpers.
 From Perennial.program_proof Require Import std_proof.
 From Perennial.goose_lang.lib Require Import waitgroup.
 
@@ -18,14 +17,14 @@ Definition own_alice ptr cli_γ next_ep hist : iProp Σ :=
   "Hown_hist" ∷ own_hist cli_γ (W64 0) sl_hist hist next_ep.
 
 Definition own_bob ptr cli_γ next_ep (ep : w64) (is_reg : bool) (pk : list w8) : iProp Σ :=
-  ∃ ptr_cli a1 a2 a3 a4 a5 sl_alicePk,
+  ∃ ptr_cli a1 a2 a3 a4 a5 sl_alicePk d0,
   "Hown_cli" ∷ client.Client.own ptr_cli
     (client.Client.mk cli_γ (W64 1) a1 next_ep a2 a3 a4 a5) ∗
   "#Hptr_cli" ∷ ptr ↦[bob :: "cli"]□ #ptr_cli ∗
   "Hptr_epoch" ∷ ptr ↦[bob :: "epoch"] #ep ∗
   "Hptr_isReg" ∷ ptr ↦[bob :: "isReg"] #is_reg ∗
   "Hptr_alicePk" ∷ ptr ↦[bob :: "alicePk"] (slice_val sl_alicePk) ∗
-  "#Hsl_alicePk" ∷ own_slice_small sl_alicePk byteT DfracDiscarded pk.
+  "Hsl_alicePk" ∷ own_slice_small sl_alicePk byteT d0 pk.
 
 Definition bob_post ptr cli_γ next_ep ep is_reg pk : iProp Σ :=
   ∃ ep',
@@ -39,14 +38,6 @@ End defs.
 Section wps.
 Context `{!heapGS Σ, !pavG Σ, !waitgroupG Σ}.
 
-Lemma wp_updAdtrsAll (servAddr : w64) sl_adtrAddrs (adtrAddrs : list w64) :
-  {{{
-    "#Hsl_adtrAddrs" ∷ own_slice_small sl_adtrAddrs uint64T DfracDiscarded adtrAddrs
-  }}}
-  updAdtrsAll #servAddr (slice_val sl_adtrAddrs)
-  {{{ RET #(); True }}}.
-Proof. Admitted.
-
 Lemma wp_alice__run hist ptr cli_γ next_ep :
   {{{
     "Hown_al" ∷ own_alice ptr cli_γ next_ep hist
@@ -56,7 +47,36 @@ Lemma wp_alice__run hist ptr cli_γ next_ep :
     next_ep' hist', RET #();
     "Hown_al" ∷ own_alice ptr cli_γ next_ep' hist'
   }}}.
-Proof. Admitted.
+Proof.
+  iIntros (Φ) "H HΦ". iNamed "H". rewrite /alice__run.
+  wp_apply wp_ref_to; [val_ty|]. iIntros "* Hptr_i".
+  wp_apply (wp_forUpto
+    (λ _, ∃ next_ep' hist', own_alice ptr cli_γ next_ep' hist')%I
+    with "[] [$Hown_al $Hptr_i]"); [word|..].
+  { clear. iIntros (? Φ) "!> H HΦ". iDestruct "H" as "((%&%&Hown_al)&Hptr_i&%)".
+    wp_apply wp_Sleep. wp_apply wp_SliceSingleton; [val_ty|]. iIntros (?) "Hsl_pk".
+    iNamed "Hown_al". wp_loadField.
+    wp_apply (wp_Client__Put with "[$Hown_cli Hsl_pk]").
+    { iApply own_slice_to_small. instantiate (1:=[(W8 1)]). iFrame "Hsl_pk". }
+    iIntros "* H". iNamed "H". simpl in *. wp_pures. wp_loadField.
+    wp_apply wp_Assume. iIntros "%Herr".
+    apply negb_true_iff in Herr. rewrite Herr. iNamed "H".
+    wp_apply wp_allocStruct; [val_ty|]. iIntros (?) "Hptr_e".
+    wp_loadField. iNamed "Hown_hist".
+    wp_apply (wp_SliceAppend with "Hsl_hist"). iIntros (?) "Hsl_hist".
+    wp_storeField.
+
+    iApply "HΦ".
+    iMod (struct_pointsto_persist with "Hptr_e") as "#Hptr_e".
+    iDestruct (struct_fields_split with "Hptr_e") as "H". iNamed "H".
+    iMod (own_slice_small_persist with "Hsl_pk") as "#Hsl_pk".
+    iDestruct (hist_extend_put with "[$His_hist $His_key]") as "His_hist_new"; [word..|].
+    iFrame "Hptr_i Hptr_hist Hptr_cli Hsl_hist His_hist_new".
+    rewrite length_app. simpl.
+    replace (W64 (length hist' + 1)%nat) with (word.add (W64 1) (W64 $ length hist')) by word.
+    iFrame "Hown_cli". iApply big_sepL2_snoc. by iFrame "#". }
+  iIntros "((%&%&Hown_al)&_)". wp_pures. by iApply ("HΦ" $! next_ep' hist').
+Qed.
 
 Lemma wp_bob__run ptr cli_γ next_ep ep is_reg pk :
   {{{
@@ -67,7 +87,14 @@ Lemma wp_bob__run ptr cli_γ next_ep ep is_reg pk :
     next_ep' ep' is_reg' pk', RET #();
     "Hbob_post" ∷ bob_post ptr cli_γ next_ep' ep' is_reg' pk'
   }}}.
-Proof. Admitted.
+Proof.
+  iIntros (Φ) "H HΦ". iNamed "H". iNamed "Hown_bob". rewrite /bob__run.
+  wp_apply wp_Sleep. wp_loadField. wp_apply (wp_Client__Get with "Hown_cli").
+  iIntros "* H". iNamed "H". wp_loadField. iClear "Herr".
+  wp_apply wp_Assume. iIntros "%Herr".
+  apply negb_true_iff in Herr. rewrite Herr. iNamed "H". do 3 wp_storeField.
+  iApply "HΦ". iFrame "∗#". word.
+Qed.
 
 Lemma wp_testAll ptr_setup setup :
   {{{
@@ -110,7 +137,7 @@ Proof using Type*.
   { iIntros "!>".
     wp_apply (wp_bob__run with "[$Hown_cli_bob $Hptr_cli_bob $epoch $isReg alicePk]").
     { iExists Slice.nil. iFrame.
-      iApply own_slice_to_small. iApply own_slice_zero. }
+      iExists (DfracOwn 1). iApply own_slice_to_small. iApply own_slice_zero. }
     iIntros "*". iNamed 1.
     by wp_apply (wp_WaitGroup__Done with "[$His_wg $Hown_tok1 $Hbob_post //]"). }
 
